App as function

TM/Code/ListTM.v
@@ -491,53 +491,39 @@ Require Import TM.Basic.Mono TM.Code.Copy.
 
 
 
-(* TODO: ~> base *)
 Lemma pair_eq (A B : Type) (a1 a2 : A) (b1 b2 : B) :
   (a1, b1) = (a2, b2) ->
   a1 = a2 /\ b1 = b2.
 Proof. intros H. now inv H. Qed.
 
 
-(* TODO: This is probably broken; is this cheat ok here? *)
-(* I think we have to copy the first list to the left of the second list, to avoid writing over the right boundary *)
-
-(** I don't use the [Computes2] Relation here, because I don't want to copy the full first list here. I simply copy memory instead of using constructors/deconstructors, which could be tedious here. *)
+(** I simply copy memory instead of using constructors/deconstructors, which could be tedious here. *)
 Section Append.
 
   Variable (sigX : finType) (X : Type) (cX : codable sigX X).
   Hypothesis (defX: inhabitedC sigX).
 
-  Notation tau := (FinType (EqType (sigList sigX))) (only parsing).
+  Notation sigList := (FinType (EqType (sigList sigX))) (only parsing).
 
-  Definition App_Rel : Rel (tapes tau^+ 2) (unit * tapes tau^+ 2) :=
+  Let stop : sigList^+ -> bool :=
+    fun x => match x with
+          | inl (START) => true (* halt at the start symbol *)
+          | _ => false
+          end.
+
+  Definition App'_Rel : Rel (tapes sigList^+ 2) (unit * tapes sigList^+ 2) :=
     ignoreParam (fun tin tout =>
                    forall (xs ys : list X),
                      tin[@Fin0] ≃ xs ->
                      tin[@Fin1] ≃ ys ->
-                     tout[@Fin0] ≃ xs ++ ys /\
-                     tout[@Fin1] ≃ ys).
-
-  Let stop : tau^+ -> bool :=
-    fun x => match x with
-          | inl (STOP) => true (* halt at the stop symbol *)
-          | _ => false
-          end.
-
-  Definition App : { M : mTM tau^+ 2 & states M -> unit } :=
-    Inject (MoveRight _;; Move L tt) [|Fin0|];;
-    Inject (Move R tt) [|Fin1|];;
-    Inject (CopySymbols stop id) [|Fin1;Fin0|];;
-    Inject (MoveLeft _) [|Fin0|];;
-    Inject (MoveLeft _) [|Fin1|].
+                     tout[@Fin0] ≃ xs /\
+                     tout[@Fin1] ≃ xs ++ ys).
 
 
+  Definition App' : { M : mTM sigList^+ 2 & states M -> unit } :=
+    Inject (MoveRight _;; Move L tt;; Move L tt) [|Fin0|];;
+    CopySymbols_L stop id.
 
-  (*
-  Compute encode [1;2;3].
-  Compute encode ([1;2;3] ++ [4;5;6]).
-  Compute removelast (encode [1;2;3]) ++ encode [4;5;6].
-*)
-  
   Lemma encode_list_app (xs ys : list X) :
     encode_list cX (xs ++ ys) = removelast (encode_list cX xs) ++ encode_list cX ys.
   Proof.
@@ -557,39 +543,90 @@ Section Append.
     encode_list cX xs <> nil.
   Proof. destruct xs; cbn; congruence. Qed.
 
-  (* Todo: clean up here a bit *)
+
+  (* TODO: -> base *)
+  Lemma app_or_nil (xs : list X) :
+    xs = nil \/ exists ys y, xs = ys ++ [y].
+  Proof.
+    induction xs as [ | x xs IH]; cbn in *.
+    - now left.
+    - destruct IH as [ -> | (ys&y&->) ].
+      + right. exists nil, x. cbn. reflexivity.
+      + right. exists (x :: ys), y. cbn. reflexivity.
+  Qed.
+
+  (* TODO: -> base *)
+  Lemma map_removelast (A B : Type) (f : A -> B) (l : list A) :
+    map f (removelast l) = removelast (map f l).
+  Proof.
+    induction l as [ | a l IH]; cbn in *; auto.
+    destruct l as [ | a' l]; cbn in *; auto.
+    f_equal. auto.
+  Qed.
 
 
-  Lemma App_Realise : App ⊨ App_Rel.
+  Lemma App'_Realise : App' ⊨ App'_Rel.
   Proof.
     eapply Realise_monotone.
-    { unfold App. repeat TM_Correct.
+    { unfold App'. repeat TM_Correct.
       - apply MoveRight_Realise with (X := list X).
-      - apply MoveLeft_Realise with (X := list X).
-      - apply MoveLeft_Realise with (X := list X).
     }
     {
-      intros tin ((), tout) H. intros xs ys HEncXS HEncYS. TMSimp; clear_trivial_eqs.
-      destruct HEncYS as (ls1&HEncYS).
-      specialize H with (1 := HEncXS). destruct H as (ls2&H). TMSimp.
-      erewrite CopySymbols_correct_moveright in H1; cbn; auto; swap 1 2.
-      { intros ? (?&<-&?) % in_map_iff. cbn. reflexivity. }
-      apply pair_eq in H1 as (H1&H1'); TMSimp.
-      specialize (H3 (xs++ys)); spec_assert H3.
-      { repeat econstructor. cbn. rewrite !map_id, <- !map_rev. cbv [id].
-        f_equal; swap 1 2.
-        + simpl_tape. rewrite map_length. destruct ys; cbn. reflexivity. apply skipn_nil.
-        + rewrite encode_list_app. rewrite rev_app_distr, map_app, <- app_assoc. f_equal.
-          simpl_tape. rewrite tl_app, tl_map; cbn. 
-          - f_equal. f_equal. generalize (encode_list cX xs); intros. apply tl_rev.
-          - intros [] % map_eq_nil % rev_eq_nil % encode_list_neq_nil.
-      }
-      
-      specialize (H4 ys). spec_assert H4.
-      { repeat econstructor. cbn. now rewrite <- !map_rev. }
-      auto.
+      intros tin ((), tout) H. cbn. intros xs ys HEncXs HEncYs.
+      destruct HEncXs as (ls1&HEncXs), HEncYs as (ls2&HEncYs). TMSimp; clear_trivial_eqs.
+      rename H into HMoveRight; rename H0 into HCopy.
+      specialize (HMoveRight xs ltac:(repeat econstructor)) as (ls3&HEncXs'). TMSimp.
+
+      pose proof app_or_nil xs as [ -> | (xs'&x&->) ]; cbn in *; auto.
+      - rewrite CopySymbols_L_Fun_equation in HCopy; cbn in *. inv HCopy; TMSimp. repeat econstructor.
+      - rewrite encode_list_app in HCopy. cbn in *.
+        rewrite rev_app_distr in HCopy. rewrite <- tl_rev in HCopy. rewrite map_app, <- !app_assoc in HCopy.
+        rewrite <- tl_map in HCopy. rewrite map_rev in HCopy. cbn in *. rewrite <- app_assoc in HCopy. cbn in *.
+        rewrite !List.map_app, !List.map_map in HCopy. rewrite rev_app_distr in HCopy. cbn in *.
+        rewrite map_rev, tl_rev in HCopy.
+
+        rewrite app_comm_cons, app_assoc in HCopy. rewrite CopySymbols_L_correct_moveleft in HCopy; cbn in *; auto.
+        + rewrite rev_app_distr, rev_involutive, <- app_assoc in HCopy. inv HCopy; TMSimp.
+          * rewrite <- app_assoc, map_id. cbn. repeat econstructor.
+            -- f_equal. cbn. rewrite encode_list_app. rewrite map_app, <- app_assoc.
+               cbn.
+               f_equal.
+               ++ now rewrite rev_involutive, map_removelast.
+               ++ f_equal. now rewrite map_app, List.map_map, <- app_assoc.
+            -- f_equal. cbn. rewrite !encode_list_app. rewrite rev_app_distr, rev_involutive, <- app_assoc.
+               cbn. rewrite rev_involutive, <- app_assoc. cbn.
+               rewrite removelast_app, !map_app, <- !app_assoc, map_removelast. 2: congruence. f_equal.
+               setoid_rewrite app_assoc at 2. rewrite app_comm_cons. rewrite app_assoc. f_equal. f_equal.
+               rewrite map_removelast. cbn -[removelast]. rewrite map_app. cbn -[removelast].
+               rewrite app_comm_cons. rewrite removelast_app. 2: congruence. cbn. now rewrite List.map_map, app_nil_r.
+        + cbn.
+          intros ? [ (?&<-&?) % in_rev % in_map_iff | H % in_rev ] % in_app_iff. cbn. auto. cbn in *.
+          rewrite rev_involutive, <- map_removelast in H.
+          apply in_app_iff in H as [ (?&<-&?) % in_map_iff | [ <- | [] ] ]. all: auto.
     }
   Qed.
 
 
+  Definition App : { M : mTM sigList^+ 3 & states M -> unit } :=
+    Inject (CopyValue _) [|Fin1; Fin2|];;
+    Inject (App') [|Fin0; Fin2|].
+
+
+  Lemma App_Computes : App ⊨ Computes2_Rel (@app X).
+  Proof.
+    eapply Realise_monotone.
+    { unfold App. repeat TM_Correct.
+      - apply CopyValue_Realise with (X := list X).
+      - apply App'_Realise.
+    }
+    {
+      intros tin ((), tout) H. cbn. intros xs ys HEncXs HEncYs HOut _.
+      TMSimp. rename H into HCopy; rename H0 into HComp.
+      specialize HCopy with (1 := HEncYs) (2 := HOut) as (HCopy1&HCopy2).
+      specialize HComp with (1 := HEncXs) (2 := HCopy2) as (HComp1&HComp2).
+      repeat split; auto.
+      - intros i; destruct_fin i.
+    }
+  Qed.
+  
 End Append.
